

#3 [6.5]: Let  $A$  and  $\vec{b}$  be the matrices below for the system  $A\vec{x} = \vec{b}$

$$A = \begin{pmatrix} 1 & -2 \\ -1 & 2 \\ 0 & 3 \\ 2 & 5 \end{pmatrix}, \quad \vec{b} = \begin{pmatrix} 3 \\ 1 \\ -4 \\ 2 \end{pmatrix}$$

(a) Construct the normal equation for  $\hat{x}$

**Solution:** Begin by noticing that the system is inconsistent and so we must approximate the solution using the least squares method:  $A^T A \hat{x} = A^T \vec{b}$  where  $\hat{x}$  is the vector such that  $\|b - A\hat{x}\| \leq \|b - A\vec{x}\|$  for all other  $\vec{x}$ . We start by finding  $A^T A$  and  $A^T \vec{b}$ :

$$A^T A = \begin{pmatrix} 6 & 6 \\ 6 & 42 \end{pmatrix}$$

$$A^T \vec{b} = \begin{pmatrix} 6 \\ -6 \end{pmatrix}$$

We can now setup the normal equations for  $\hat{x}$ :

$$\begin{pmatrix} 6 & 6 \\ 6 & 42 \end{pmatrix} \begin{pmatrix} x_1 \\ x_2 \end{pmatrix} = \begin{pmatrix} 6 \\ -6 \end{pmatrix}$$

(b) Solve for  $\hat{x}$

**Solution:** To solve for  $\hat{x}$  we can first notice that  $(A^T A)^{-1}$  exists since  $\det A^T A = 216 \neq 0$ . Thus, using the formula for the inverse of a  $2 \times 2$  matrix we have

$$(A^T A)^{-1} = \frac{1}{216} \begin{pmatrix} 42 & -6 \\ -6 & 6 \end{pmatrix}.$$

Now,

$$A^T A \hat{x} = A^T \vec{b} \Rightarrow \hat{x} = (A^T A)^{-1} (A^T \vec{b}).$$

Thus, using our calculation of  $A^T \vec{b}$  from part (a), we have

$$\hat{x} = \frac{1}{216} \begin{pmatrix} 42 & -6 \\ -6 & 6 \end{pmatrix} \begin{pmatrix} 6 \\ -6 \end{pmatrix} = \frac{1}{216} \begin{pmatrix} 288 \\ -72 \end{pmatrix} = \begin{pmatrix} 4/3 \\ -1/3 \end{pmatrix}$$

#7 [7.1]: Determine if the matrix below is orthogonal. If it is, find the inverse.

$$\begin{pmatrix} .6 & .8 \\ .8 & -.6 \end{pmatrix}$$

**Solution:** Recall the definition of an orthogonal matrix is a matrix  $Q$  such that  $Q^T Q = I$ . We can check if the above matrix is orthogonal using this definition:

$$\begin{pmatrix} .6 & .8 \\ .8 & -.6 \end{pmatrix} \begin{pmatrix} .6 & .8 \\ .8 & -.6 \end{pmatrix} = \begin{pmatrix} 1 & 0 \\ 0 & 1 \end{pmatrix}.$$

Therefore, by definition, the above matrix **is orthogonal**. Thus, the inverse is simply the transpose, if the above matrix is  $Q$ , then

$$Q^T = Q^{-1} = \begin{pmatrix} .6 & .8 \\ .8 & -.6 \end{pmatrix}$$

**#17 [7.1]:** Orthogonally diagonalize the matrix given below with eigenvalues  $\lambda = -4, 4, 7$

$$A = \begin{pmatrix} 1 & 1 & 5 \\ 1 & 5 & 1 \\ 5 & 1 & 1 \end{pmatrix}$$

**Solution:** We start by finding the eigenvectors. For  $\lambda = -4$  we have

$$\begin{aligned} A + 4I &= \begin{pmatrix} 5 & 1 & 5 \\ 1 & 9 & 1 \\ 5 & 1 & 4 \end{pmatrix} \xrightarrow{R_1 \leftrightarrow R_2} \begin{pmatrix} 1 & 9 & 1 \\ 5 & 1 & 5 \\ 5 & 1 & 5 \end{pmatrix} \xrightarrow{R_3 \rightarrow R_3 - R_2} \begin{pmatrix} 1 & 9 & 1 \\ 5 & 1 & 5 \\ 0 & 0 & 0 \end{pmatrix} \xrightarrow{R_2 \rightarrow R_2 - 5R_1} \begin{pmatrix} 1 & 9 & 1 \\ 0 & -44 & 0 \\ 0 & 0 & 0 \end{pmatrix} \\ \Rightarrow X &= t \begin{pmatrix} -1 \\ 0 \\ 1 \end{pmatrix} \Rightarrow \vec{u}_1 = \begin{pmatrix} -1/\sqrt{2} \\ 0 \\ 1/\sqrt{2} \end{pmatrix} \end{aligned}$$

Now for  $\lambda = 4$ :

$$\begin{aligned} A - 4I &= \begin{pmatrix} -3 & 1 & 5 \\ 1 & 1 & 1 \\ 5 & 1 & -3 \end{pmatrix} \xrightarrow{R_2 \leftrightarrow R_1} \begin{pmatrix} 1 & 1 & 1 \\ -3 & 1 & 5 \\ 5 & 1 & -3 \end{pmatrix} \xrightarrow[R_3 \rightarrow R_3 - 5R_1]{R_2 \rightarrow R_2 + 3R_1} \begin{pmatrix} 1 & 1 & 1 \\ 0 & 4 & 8 \\ 0 & -4 & -8 \end{pmatrix} \xrightarrow{R_3 \rightarrow R_3 + R_2} \begin{pmatrix} 1 & 1 & 1 \\ 0 & 4 & 8 \\ 0 & 0 & 0 \end{pmatrix} \\ \Rightarrow X &= t \begin{pmatrix} 1 \\ -2 \\ 1 \end{pmatrix} \Rightarrow \vec{u}_2 = \begin{pmatrix} 1/\sqrt{6} \\ -2/\sqrt{6} \\ 1/\sqrt{6} \end{pmatrix} \end{aligned}$$

For  $\lambda = 7$ :

$$\begin{aligned} A - 7I &= \begin{pmatrix} -6 & 1 & 5 \\ 1 & -2 & 1 \\ 5 & 1 & -6 \end{pmatrix} \xrightarrow{R_2 \leftrightarrow R_1} \begin{pmatrix} 1 & -2 & 1 \\ -6 & 1 & 5 \\ 5 & 1 & -6 \end{pmatrix} \xrightarrow[R_3 \rightarrow R_3 - 5R_1]{R_2 \rightarrow R_2 + 6R_1} \begin{pmatrix} 1 & -1 & 1 \\ 0 & -11 & 11 \\ 0 & 11 & -11 \end{pmatrix} \\ \xrightarrow{R_3 \rightarrow R_3 + R_2} &\begin{pmatrix} 1 & -1 & 1 \\ 0 & -11 & 11 \\ 0 & 0 & 0 \end{pmatrix} \Rightarrow X = t \begin{pmatrix} 1 \\ 1 \\ 1 \end{pmatrix} \Rightarrow \vec{u}_3 = \begin{pmatrix} 1/\sqrt{3} \\ 1/\sqrt{3} \\ 1/\sqrt{3} \end{pmatrix} \end{aligned}$$

Where  $\vec{u}_1, \vec{u}_2, \vec{u}_3$  are unit vectors in the respective eigenspaces. We can now form  $P$  and  $D$ :

$$P = \begin{pmatrix} -1/\sqrt{2} & 1/\sqrt{6} & 1/\sqrt{3} \\ 0 & -2/\sqrt{6} & 1/\sqrt{3} \\ 1/\sqrt{2} & 1/\sqrt{6} & 1/\sqrt{3} \end{pmatrix}, \quad D = \begin{pmatrix} -4 & 0 & 0 \\ 0 & 4 & 0 \\ 0 & 0 & 7 \end{pmatrix}$$

**#5 [7.2]:** Find the matrix of the quadratic form. Assume  $\vec{x} \in \mathbb{R}^3$ .

(a)  $3x_1^2 + 2x_2^2 - 5x_3^2 - 6x_1x_2 + 8x_1x_3 - 4x_2x_3$

**Solution:** Denote the above quadratic form as  $Q(\vec{x})$ . The coefficients of the quadratic terms correspond to the main diagonal of the matrix. The coefficients of the cross-product terms correspond to twice the  $(i, j)$  and  $(j, i)$  entries. With this in mind we can form the matrix as follows,

$$\begin{pmatrix} 3 & -3 & 4 \\ -3 & 2 & -2 \\ 4 & -2 & -5 \end{pmatrix}$$

(b)  $6x_1x_2 + 4x_1x_3 - 10x_2x_3$

**Solution:** We can use similar logic to part (a) while noticing that there are no quadratic terms so all the diagonal entries are 0. Thus, the corresponding matrix is

$$\begin{pmatrix} 0 & 3 & 2 \\ 3 & 0 & -5 \\ 2 & -5 & 0 \end{pmatrix}$$

**#11 [7.2]:** Classify the quadratic form  $Q(\vec{x}) = 2x_1^2 - 4x_1x_2 - x_2^2$ . Then make a change of variable,  $\vec{x} = P\vec{y}$ , that transforms the quadratic form into one with no cross-product term and write the new quadratic form.

**Solution:** Using similar logic as in problem (5) we can form the corresponding matrix as

$$A = \begin{pmatrix} 2 & -2 \\ -2 & -1 \end{pmatrix}$$

We can now find the characteristic equation of  $A$  (using the known characteristic equation for a  $2 \times 2$  matrix) and use it to find the eigenvalues:

$$\lambda^2 - \lambda - 6 \Rightarrow (\lambda - 3)(\lambda + 2) = 0 \Rightarrow \lambda = 3, -2$$

Since the eigenvalues of  $A$  are both positive and negative, we can classify  $Q$  as **indefinite**. To find the change of variable we must first find the eigenvectors of  $A$ :

For  $\lambda = 3$ :

For  $\lambda = -2$ :

$$A - 3I = \begin{pmatrix} -1 & -2 \\ -2 & -4 \end{pmatrix} \xrightarrow{R_2 \rightarrow R_2 - 2R_1} \begin{pmatrix} -1 & -2 \\ 0 & 0 \end{pmatrix}$$

$$A + 2I = \begin{pmatrix} 4 & -2 \\ -2 & 1 \end{pmatrix} \xrightarrow{R_2 \rightarrow 2R_2 + R_1} \begin{pmatrix} 4 & -2 \\ 0 & 0 \end{pmatrix}$$

$$\Rightarrow X = t \begin{pmatrix} -2 \\ 1 \end{pmatrix} \Rightarrow \vec{u}_1 = \begin{pmatrix} -2/\sqrt{3} \\ 1/\sqrt{3} \end{pmatrix}$$

$$\Rightarrow X = t \begin{pmatrix} 1 \\ 2 \end{pmatrix} \Rightarrow \vec{u}_2 = \begin{pmatrix} 1/\sqrt{3} \\ 2/\sqrt{3} \end{pmatrix}$$

Using the unit vectors  $\vec{u}_1$  and  $\vec{u}_2$ , as well as  $\lambda_1 = 3$  and  $\lambda_2 = -2$  we can form  $P$  (since the set  $\{\vec{u}_1, \vec{u}_2\}$  is orthogonal) and  $D$ :

$$P = \begin{pmatrix} -2/\sqrt{3} & 1/\sqrt{3} \\ 1/\sqrt{3} & 2/\sqrt{3} \end{pmatrix}, \quad D = \begin{pmatrix} 3 & 0 \\ 0 & -2 \end{pmatrix}.$$

Performing the change of variables  $\vec{x} = P\vec{y}$  gives the new quadratic form of

$$\vec{y}^T D \vec{y} = \boxed{3y_1^2 - 2y_2^2}$$